Phi_Semantics/PhiSem_Mem_C.thy
@@ -212,14 +212,19 @@ proc op_free_mem:
 
 \<medium_right_bracket> .
  
-declare [[\<phi>trace_reasoning = 0]]
+declare [[\<phi>trace_reasoning = 3]]
+
+declare hd_zip[simp]
+
+
+declare length_Suc_conv[simp]
 
 \<phi>type_def Mem_Slice :: \<open>logaddr \<Rightarrow> nat len_intvl \<Rightarrow> (mem_fic,'a) \<phi> \<Rightarrow> (fiction, 'a list) \<phi>\<close>
   where \<open>l \<Ztypecolon> Mem_Slice addr iv T \<equiv>
           zip [len_intvl.start iv ..< len_intvl.start iv + len_intvl.len iv] l
             \<Ztypecolon> \<big_ast>\<^sub>\<lbrakk>\<^sub>:\<^sub>\<rbrakk>\<^sup>\<phi> iv (\<Sigma> j. \<m>\<e>\<m>[addr \<tribullet>\<^sub>a j\<^sup>\<t>\<^sup>\<h>] T) \<s>\<u>\<b>\<j> length l = len_intvl.len iv\<close>
     \<comment> \<open>Length is still required because it determines the domain of the \<phi>-type so guides the reasoning\<close>
-  deriving Sep_Functor_1
+  deriving (*Sep_Functor_1
        and \<open>Abstract_Domain T P
         \<Longrightarrow> Abstract_Domain (Mem_Slice addr iv T) (\<lambda>x. length x = len_intvl.len iv \<and> list_all P x) \<close>
             tactic: (cases iv; simp add: list_all_length)
@@ -239,6 +244,9 @@ declare [[\<phi>trace_reasoning = 0]]
             tactic: (clarsimp simp add: list_all2_conv_all_nth unzip'_def)
        and Semimodule_SDistr_Homo
        and Semimodule_Zero
+       and*) \<open>Semimodule_One (Mem_Slice addr) T (\<m>\<e>\<m>[addr \<tribullet>\<^sub>a j\<^sup>\<t>\<^sup>\<h>] T) \<lbrakk>j:1\<rwpar> (\<lambda>l. length l = 1) hd\<close>
+
+term \<open>Semimodule_One (Mem_Slice addr) T (\<m>\<e>\<m>[addr \<tribullet>\<^sub>a j\<^sup>\<t>\<^sup>\<h>] T) \<lbrakk>j:1\<rwpar> (\<lambda>_. True) hd\<close>
 
 term \<open>Semimodule_SDistr_Homo\<^sub>Z (Mem_Slice addr) T (\<lambda>_. True) \<close>
 
